src/Simulation.v
@@ -163,5 +163,9 @@ Section InvSim.
   
 End InvSim.
 
+Definition liftSim {iifc sifc} (ossSim: OStates iifc -> OStates sifc -> Prop):
+  MState iifc -> MState sifc -> Prop :=
+  fun ist sst => ossSim (bst_oss ist) (bst_oss sst).
+
 Close Scope list.
 
